\begin{algorithm}[t]
\begin{gather*}
\begin{aligned}
&\text{Ex. Kalman Filter}                           &       &\text{Ex. Information Filter} \\
&                                                   &       H_n &= \left(P_n\right)^{-1} \\
K_n &= P_n^0 J_n^T(J_n P_n^0 J_n^T + R)^{-1}        &       H_n &= H_n^0 + J_n^T R^{-1} J_n \\
\hat{x}_n &= \hat{x}_n^0 + K_n(z_n - F_n)           &       K_n &= {H_n}^{-1} J_n^T R^{-1} \\
P_n &= (I - K_n J_n)P_n^0                           &       \hat{x}_n &= \hat{x}_n^0 + K_n (z_n - F_n)
\end{aligned}
\end{gather*}
\caption{
% 
% 
Analogy of EKF and EIF.
% 
% 
}
\label{tab:eif}
\end{algorithm}