\begin{algorithm}[b]
\vspace{-.1in}
\begin{align*}
&\text{for} \quad i=1... i_{\text{max}} \\
& \quad \quad
\begin{aligned}
F_n^i &= F(\hat{x}_n^i) \Rightarrow {J_n^i}_{[u, v]} = {\partial F^i_{[u]}}(\hat{x}_n^i)/{\partial x_{[v]}} \\
K_n^i &= P_n^0 {J^{iT}_n}(J_n^i P_n^0 {J^{iT}_n} + R)^{-1} \\
\hat{x}_n^{i+1} &= \hat{x}_n^0 + K_n^i(z_n - F_n^i -J_n^i(\hat{x}_n^0 - \hat{x}_n^i)) \\
\end{aligned} 
\\
& \text{end} \\
& \hat{x}_n = \hat{x}_n^i \\   
& P_n = (I - K_n^\textit{\color{accent}$i$} J_n^i) P_n^0
\end{align*}
\caption{Iterated EKF measurement update equations.}
\label{tab:iekf}
\end{algorithm}

\endinput % IGNORES WHAT FOLLOWS
%%%%%%%%%%%%%%%%%%%%%%%%%%%%%%%%%%%%%%%%%%%%%%%%%%%%%%%%%%%%%%%%%%%%%%%%
%%%%%%%%%%%%%%%%%%%%%%%%%%%%%%%%%%%%%%%%%%%%%%%%%%%%%%%%%%%%%%%%%%%%%%%%
%%%%%%%%%%%%%%%%%%%%%%%%%%%%%%%%%%%%%%%%%%%%%%%%%%%%%%%%%%%%%%%%%%%%%%%%
%%%%%%%%%%%%%%%%%%%%%%%%%%%%%%%%%%%%%%%%%%%%%%%%%%%%%%%%%%%%%%%%%%%%%%%%
%%%%%%%%%%%%%%%%%%%%%%%%%%%%%%%%%%%%%%%%%%%%%%%%%%%%%%%%%%%%%%%%%%%%%%%%
%%%%%%%%%%%%%%%%%%%%%%%%%%%%%%%%%%%%%%%%%%%%%%%%%%%%%%%%%%%%%%%%%%%%%%%%
%%%%%%%%%%%%%%%%%%%%%%%%%%%%%%%%%%%%%%%%%%%%%%%%%%%%%%%%%%%%%%%%%%%%%%%%

\begin{table}[h] 
\centering
\resizebox{0.48\textwidth}{!}{
\begin{tabular}{|l|l|}
\hline
Extended Kalman Filter & Iterated Extended Kalman Filter \\
\hline
&
for $i = 1...$ \\
  
$F_n = F(\hat{x}_n^0)$ &
$\:\:\: F_n^\textit{\color{accent}$i$} = F( \hat{x}_n^\textit{\color{accent}$i$})$ \\

${J_n}_{[u, v]} = \frac{ \partial F_{[u]}}{ \partial x_{[v]}}(\hat{x}_n^0)$ & 
$\:\:\: {J_n}_{[u, v]}^\textit{\color{accent}$i$} = \frac{ \partial F_{[u]}^\textit{\color{accent}$i$}}{ \partial x_{[v]}}(\hat{x}_n^\textit{\color{accent}$i$})$\\

$K_n = P_n^0 J_n^T(J_n P_n^0 J_n^T + R)^{-1}$ &
$\:\:\: K_n^\textit{\color{accent}$i$} = P_n^0 {J^\textit{\color{accent}$i$}_n}^T(J_n^\textit{\color{accent}$i$} P_n^0 {J^\textit{\color{accent}$i$}_n}^T + R)^{-1}$ \\

$\hat{x}_n = \hat{x}_n^0 + K_n(z_n - F_n)$ &
$\:\:\: \hat{x}_n^\textit{\color{accent}$i + 1$} = \hat{x}_n^0 + K_n^\textit{\color{accent}$i$}(z_n - F_n^\textit{\color{accent}$i$} - $\\

 &$\:\:\:\:\:\:\:\:\:\:\:\: - \textit{\color{accent} $J_n^i(\hat{x}_n^0 - \hat{x}_n^i)$})$ \\

 &
end \\
 
 & $\hat{x}_n = \hat{x}_n^\textit{\color{accent}$i$}$ \\
 
$P_n = (I - K_n J_n)P_n^0$ &
$P_n = (I - K_n^\textit{\color{accent}$i$} J_n^\textit{\color{accent}$i$})P_n^0$ \\

\hline
\end{tabular}
}
\caption{EKF vs. IEKF measurement update equations \label{tab:ekf-iekf}}
\end{table}